LynxTest.lean
@@ -1,14 +1,11 @@
-import LynxTest.Integration.Sum
+import LynxTest.Integration
 import LynxTest.Term
 import LynxTest.Term.Compare
 import LynxTest.Term.Map
-import LynxTest.Integration.Reverse
 import LynxTest.Tactic.Contracts
 import LynxTest.Tactic.Recursive
 import LynxTest.Tactic.Opaque
 import LynxTest.Tactic.Failures
-import LynxTest.ProofAudit
 import LynxTest.Modules.Extensions
 import LynxTest.Modules.Erlang
-import LynxTest.Integration.Sets
 import LynxTest.Modules.Maps
